Flesh out definability theorems

closures/BohmTrees.v
@@ -6,19 +6,26 @@ Require Import Lambda.
 Inductive hnf : Ob -> Type :=
   | hnf_TOP: hnf TOP
   | hnf_K: hnf K
-  | hnf_Kx x: hnf (K * x)
+  | hnf_Kx x: definable x -> hnf (K * x)
   | hnf_S: hnf S
   | hnf_Sx x: hnf x -> hnf (S * x)
-  | hnf_Sxy x y: hnf x -> hnf (S * x * y)
+  | hnf_Sxy x y: hnf x -> definable y -> hnf (S * x * y)
   | hnf_Rxy x y: hnf x -> hnf y -> hnf (x(+)y)
   | hnf_Jxy x y: hnf x -> hnf y -> hnf (x||y)
-  | hnf_Join (s : Set) (e : s -> Ob): (forall i, hnf (e i)) -> hnf (Join e).
+(*| hnf_Join (s : Set) (e : s -> Ob): (forall i, hnf (e i)) -> hnf (Join e)*)
+.
 Hint Constructors hnf.
 
-Theorem hnf_conv: forall x : Ob, conv x -> {y : Ob & y [= x & hnf y}.
+Lemma hnf_definable: forall x, hnf x -> definable x.
 Proof.
-  intros x Hconv.
+  intros x H; induction H; auto.
+Qed.
+
+Theorem hnf_conv:
+  forall f x : Ob, conv (f * x) ->
+  {y : Ob & y [= x & ((hnf y) * (conv (f * y)))%type}.
+Proof.
+  intros f x Hconv.
   inversion Hconv.
-    exists TOP; auto.
   (* TODO *)
 Admitted.
