closures/Lambda.v
@@ -36,10 +36,10 @@ Section Encode.
     | y => false
     end.
 
-  (* Simple [I,K,S] abstraction *)
+  (* Simple [K,S] abstraction *)
   Fixpoint abstract0 (n : nat) (x : Lambda) : Lambda :=
     match x with
-    | VAR m => if beq_nat m n then [I] else [K] [*] x
+    | VAR m => if beq_nat m n then [S*K*K] else [K] [*] x
     | ABS m y => if beq_nat m n then [K] [*] x else ABS m (abstract0 n y)
     | APP y z => [S] [*] (abstract0 n y) [*] (abstract0 n z)
     | _ => [K] [*] x
@@ -62,10 +62,10 @@ Section Encode.
     | _ => [K] [*] x
     end.
 
-  Fixpoint compile (x : Lambda) : Lambda :=
+  Fixpoint compile (a : nat -> Lambda -> Lambda) (x : Lambda) : Lambda :=
     match x with
-    | APP y z => APP (compile y) (compile z)
-    | ABS n y => abstract n (compile y)
+    | APP y z => APP (compile a y) (compile a z)
+    | ABS n y => a n (compile a y)
     | y => y
     end.
 
@@ -76,7 +76,8 @@ Section Encode.
     | _ => TOP
     end.
 
-  Definition encode x := close (compile x).
+  Definition encode0 x := close (compile abstract0 x).
+  Definition encode x := close (compile abstract x).
 End Encode.
 
 Notation "[ x ]" := (OB x) : Lambda_scope.
@@ -102,6 +103,26 @@ Notation "x || y" := ([J] * x * y)%Lambda
 Notation "x (+) y" := ([R] * x * y)%Lambda
   (at level 45, no associativity) : Lambda_scope.
 
+Section I_def.
+  Let x := VAR 0.
+  Let y := VAR 1.
+  Let z := VAR 2.
+
+  Lemma I_def: I = encode0 (\x, x). beta_eta. Qed.
+  Lemma F_def: F = encode0 (\x,\y, y). beta_eta. Qed.
+  Lemma B_def: B = encode0 (\x,\y,\z, x * (y * z)). beta_eta. Qed.
+  Lemma C_def: C = encode0 (\x,\y,\z, x * z * y). beta_eta. Qed.
+  Lemma W_def: W = encode0 (\x,\y, x * y * y). beta_eta. Qed.
+End I_def.
+
+Lemma I_definable: definable I. rewrite I_def; compute; auto. Qed.
+Lemma F_definable: definable F. rewrite F_def; compute; auto. Qed.
+Lemma B_definable: definable B. rewrite B_def; compute; auto 100. Qed.
+Lemma C_definable: definable C. rewrite C_def; compute; auto 100. Qed.
+Lemma W_definable: definable W. rewrite W_def; compute; auto 100. Qed.
+
+Hint Resolve I_definable F_definable B_definable C_definable W_definable.
+
 (** ** A standard library *)
 
 Section Y.
@@ -109,9 +130,10 @@ Section Y.
   Let y := VAR 1.
   Definition Y := encode (\x, (\y, x*(y*y)) * (\y, x*(y*y))).
 End Y.
+Lemma Y_definable: definable Y. compute; auto. Qed.
 Lemma Y_fix : forall f : Ob, Y*f = f*(Y*f).
 Proof.
-  intros. unfold Y. compute.
+  intros; unfold Y; compute.
   rewrite S_beta at 1.
   rewrite C_beta at 1.
   rewrite B_beta at 1.
@@ -133,6 +155,7 @@ Section V.
   Definition V_prefix := encode (\x,\y, [I] || y o (x * y)).
   Definition V := Y * V_prefix.
 End V.
+Lemma V_definable: definable V. compute; auto 100. Qed.
 Lemma V_fix : forall f : Ob, f o (V*f) [= V*f.
 Proof.
   intros f.
@@ -141,6 +164,22 @@ Proof.
   unfold V_prefix.
   auto.
 Qed.
+
+Definition TOP_def := V * K.
+Lemma TOP_TOP_def: TOP = TOP_def.
+Proof.
+  apply LESS_antisym.
+    unfold TOP_def.
+    apply LESS_conv; intros f Hconv.
+    admit. (* TODO *)
+  auto.
+Qed.
+
+Theorem TOP_definable: definable TOP.
+Proof.
+  rewrite TOP_TOP_def; compute; auto 100.
+Qed.
+Hint Resolve TOP_definable.
 
 Section div.
   Let x := VAR 0.
@@ -166,6 +205,4 @@ End exp.
 Notation "x --> y" := ([exp] * x * y)%Lambda
   (at level 55, right associativity) : Lambda_scope.
 Lemma exp_I_I: exp * I * I = I.
-Proof.
-  compute; eta_expand; eta_expand; beta_reduce; auto.
-Qed.
+Proof. beta_eta. Qed.
